Removed remaining admits

easycrypt/KEM.ec
@@ -84,7 +84,6 @@ theory Agile_Labeled_KEM.
     }.
   
     module W = {
-      var pk : pkey
       var sk : skey
       var keys : key set
       var labels : label set
@@ -112,13 +111,14 @@ theory Agile_Labeled_KEM.
         var k0, k1 : key;
         var c : ciphertext;
         var t : label;
+        var pk : pkey;
         KEM.init();
-        (W.pk, W.sk) = KEM.keygen();
+        (pk, W.sk) = KEM.keygen();
         W.keys = FSet.empty;
         W.labels = FSet.empty;
-        t = A.choose(W.pk);
+        t = A.choose(pk);
         valid = !mem t W.labels; 
-        (k0, c) = KEM.enc(pp, W.pk, t);
+        (k0, c) = KEM.enc(pp, pk, t);
         k1 = $key;
         b = ${0,1};
         W.keys = add k0 (add k1 W.keys);
@@ -310,12 +310,10 @@ section.
     {RO_KEF, RCCA, PCA.NR_PCA, PCA.OW_PCA}.
 
   (* Assumptions about the Pre-master secret KEM *)
-  axiom lossless_dec : islossless PMS_KEM.dec.
-
   (* TODO: remove this *)
   axiom stateless_pms_kem : forall (x y:glob PMS_KEM), x = y.
   
-  pred keypair : (pkey * skey).
+  op keypair : pkey * skey -> bool.
 
   op decrypt : skey -> version -> ciphertext -> pms.
   
@@ -323,7 +321,7 @@ section.
   axiom dec_injective_pv : forall sk pv1 pv2 c,
     decrypt sk pv1 c = decrypt sk pv2 c => pv1 = pv2.
 
-  axiom keygen_rel :
+  axiom keygen_spec_rel :
     equiv [ PMS_KEM.keygen ~ PMS_KEM.keygen : 
       true ==> ={res} /\ keypair res{1} ].
 
@@ -331,12 +329,12 @@ section.
     equiv [ PMS_KEM.enc ~ PMS_KEM.enc :
       pk{1} = pk /\ t{1} = pv /\ ={pk, t} /\ keypair(pk, sk) ==>
       ={res} /\ let (k, c) = res{1} in decrypt sk pv c = k ].
-  
-  axiom dec_spec_rel : forall sk pv c,
-    equiv [ PMS_KEM.dec ~ PMS_KEM.dec :
-      sk{1} = sk /\ t{1} = pv /\ c{1} = c /\ ={sk, t, c} ==>
-      ={res} /\ res{1} = decrypt sk pv c ].
-  
+
+  axiom enc_spec : forall _sk _pk _pv,
+    bd_hoare [ PMS_KEM.enc :
+      pk = _pk /\ t = _pv /\ keypair(_pk, _sk) ==>
+      let (k, c) = res in decrypt _sk _pv c = k ] = 1%r.
+ 
   axiom dec_spec : forall _sk _pv _c,
     bd_hoare [ PMS_KEM.dec :
       sk = _sk /\ t = _pv /\ c = _c ==> res = decrypt _sk _pv _c ] = 1%r.
@@ -355,6 +353,87 @@ section.
   axiom lossless_guess : 
     forall (O1 <: KEF.Oracle {A}) (O2 <: Oracle {A}),
       islossless O2.dec => islossless O1.extract => islossless A(O1, O2).guess.
+   
+  local module RCCA0 = {
+    module O = {
+      fun dec(p:version * hash, t:label, c:ciphertext) : ms option = {
+        var pv : version;
+        var h : hash;
+        var pms : pms;
+        var k : ms;
+        var maybe_k : ms option = None;
+        if (!mem t W.labels /\ mem p P) { 
+          W.labels = add t W.labels;
+          (pv, h) = p;
+          pms = decrypt W.sk pv c;
+          k = RO_KEF.extract(h, (pms, t));
+          maybe_k = if (!mem k W.keys) then Some k else None;
+        }
+        return maybe_k;
+      }
+    }
+
+    module A = A(RO_KEF, O)
+
+    fun main() : bool = {
+      var b, b', valid : bool;
+      var k0, k1 : ms;
+      var c : ciphertext;
+      var t : label;
+      var pk : pkey;
+      var pv : version;
+      var pms : pms;
+      var h : hash;
+      MS_KEM.init();
+      (pk, W.sk) = MS_KEM.keygen();
+      W.keys = FSet.empty;
+      W.labels = FSet.empty;
+      (pv, h) = pp;
+      (pms, c) = PMS_KEM.enc((), pk, pv);
+      t = A.choose(pk);
+      valid = !mem t W.labels;
+      k0 = RO_KEF.extract(h, (pms, t));
+      k1 = $key;
+      b = ${0,1};
+      W.keys = add k0 (add k1 W.keys);
+      b' = A.guess(c, if b then k1 else k0);
+      return (b = b' /\ valid);
+    }
+  }.
+
+  local equiv RCCA_RCCA0_dec :
+    RCCA(MS_KEM, A(RO_KEF)).O.dec ~ RCCA0.O.dec : 
+    ={p, t, c} /\ ={glob W, glob RO_KEF} ==>
+    ={res} /\ ={glob W, glob RO_KEF}.
+  proof.
+    fun; sp; if => //.
+    inline KEM(RO_KEF, PMS_KEM).dec; wp; sp.
+    call (_: ={glob W, glob RO_KEF}); first by eqobs_in.
+    exists * sk{1}, pv{1}, c0{1}; elim *; intros sk pv c.
+    by call{1} (dec_spec sk pv c). 
+  qed.    
+   
+  local equiv RCCA_RCCA0 : 
+    RCCA(MS_KEM, A(RO_KEF)).main ~ RCCA0.main : true ==> ={res}.
+  proof.
+    fun.
+    swap{2} [5..6] 1.
+    call (_: ={glob W, glob RO_KEF}).
+      by apply RCCA_RCCA0_dec.
+      by fun; eqobs_in.
+    inline KEM(RO_KEF, PMS_KEM).enc.
+    wp; rnd; rnd; wp.
+    call (_: ={glob W, glob RO_KEF}); first by eqobs_in.
+    seq 5 5 : (={t, pk, glob A, glob W, glob RO_KEF} /\ keypair(pk, W.sk){1}).
+    call (_: ={glob W, glob RO_KEF}).
+      by apply RCCA_RCCA0_dec.
+      by fun; eqobs_in.
+    inline KEM(RO_KEF, PMS_KEM).init KEM(RO_KEF, PMS_KEM).keygen
+           MS_KEM.init RO_KEF.init MS_KEM.keygen.
+    by wp; call keygen_spec_rel; wp; call (_:true).
+    sp; exists * W.sk{1}, pk0{1}, pv{1}; elim *; intros sk pk pv.
+    by wp; call (enc_spec_rel pk sk pv); skip; progress; smt.
+  qed.
 
   (* Global variables in RCCA1 and RCCA2 *)
   local module V = {
@@ -401,7 +480,7 @@ section.
         if (!mem t V.labels /\ mem p P) { 
           V.labels = add t V.labels;
           (pv, h) = p;
-          pms = PMS_KEM.dec((), V.sk, pv, c);
+          pms = decrypt V.sk pv c;
           abort = abort \/ (V.guess /\ pms = V.pms /\ t = V.t /\ c <> V.c);
           if (!(V.guess /\ (pv, h) = pp /\ t = V.t /\ c = V.c)) {
             if (!in_dom (h, (pms, t)) m) m.[(h, (pms, t))] = $key;
@@ -437,8 +516,8 @@ section.
    }
   }.
   
-  (** RCCA -> RCCA 1 **)
-  local equiv RCCA_RCCA1_extract_upto :
+  (** RCCA0 -> RCCA1 **)
+  local equiv RCCA0_RCCA1_extract_upto :
     RO_KEF.extract ~ RCCA1.O1.extract :
     !RCCA1.abort{2} /\
     ={p, s} /\
@@ -471,18 +550,17 @@ section.
         by rnd{2}; skip; smt.
         by skip; smt.     
       (* doesn't abort *)
-      if.
-        by smt.
+      if; first by smt.
         by wp; rnd; skip; progress; smt.    
-      wp; skip; progress.
-      cut W : 
-        (p, (pms, t)){2} <>
-        (snd pp, (decrypt V.sk (fst pp) V.c, V.t)){2} by smt.
-      by generalize H1; rewrite eq_except_def; smt.
+        wp; skip; progress.
+        cut W : 
+         (p, (pms, t)){2} <>
+         (snd pp, (decrypt V.sk (fst pp) V.c, V.t)){2} by smt.
+        by generalize H1; rewrite eq_except_def; smt.
   qed.
   
-  local equiv RCCA_RCCA1_dec_upto :
-    RCCA(MS_KEM, A(RO_KEF)).O.dec ~ RCCA1.O2.dec :
+  local equiv RCCA0_RCCA1_dec_upto :
+    RCCA0.O.dec ~ RCCA1.O2.dec :
     !RCCA1.abort{2} /\
     ={p, t, c} /\
     V.guess{2} /\
@@ -506,61 +584,39 @@ section.
       decrypt V.sk{2} (fst pp) V.c{2} = V.pms{2}.
   proof.
     fun.
-    sp; if => //.  
-    wp; inline KEM(RO_KEF, PMS_KEM).dec.
-    seq 7 3 : 
-      ((decrypt W.sk pv c0 = pms){1} /\
-       maybe_k{1} = None /\
-       sk{1} = W.sk{1} /\ c0{1} = c{2} /\ t0{1} = t{2} /\
-       ={maybe_k, pms, pv, h, p, t, c} /\
-       !RCCA1.abort{2} /\ 
-       V.guess{2} /\
-       W.sk{1} = V.sk{2} /\
-       W.keys{1} = V.keys{2} /\
-       W.labels{1} = V.labels{2} /\
-       eq_except RO_KEF.m{1} RCCA1.m{2} (snd pp, (V.pms, V.t)){2} /\
-       in_dom (snd pp, (V.pms, V.t)){2} RO_KEF.m{1} /\
-       mem (proj RO_KEF.m{1}.[(snd pp, (V.pms, V.t))]){2} V.keys{2} /\
-       decrypt V.sk{2} (fst pp) V.c{2} = V.pms{2}).
-      sp; exists * sk{1}, pv{1}, c0{1}; elim *; intros sk pv c.
-      by call (dec_spec_rel sk pv c); wp.
-   
-      wp; sp; case RCCA1.abort{2}.
-        (* aborts *)
-        call{1} (_:true ==> true); first by apply lossless_extract.
+    sp; if => //.
+    wp; sp; case RCCA1.abort{2}.
+      (* aborts *)
+      call{1} (_:true ==> true); first by apply lossless_extract.
+      if{2}.
         if{2}.
-          if{2}.
-            by wp; rnd{2}; skip; smt.
-            by wp; skip; smt.
-          by skip; smt.
-   
-        (* doesn't abort *)
-        inline{1} RO_KEF.extract.
-        if{2}.
-          wp; sp; if.
-            by progress; cut W :
-              (snd pp, (decrypt V.sk (fst pp) V.c, V.t)){2} <>
-              (h, (decrypt V.sk pv c, t)){2}; smt.   
-            by rnd; skip; progress; smt.
-      
-         skip; progress.
-         cut W :
-           (snd pp, (decrypt V.sk (fst pp) V.c, V.t)){2} <>
-           (h, (decrypt V.sk pv c, t)){2} by smt.
-         by generalize H1; rewrite eq_except_def; smt.
-   
-      wp; sp; if{1}.
-        by rnd{1}; skip; smt.
-        by skip; smt.
+          by wp; rnd{2}; skip; smt.
+          by wp; skip; smt.
+        by skip; smt.    
+      (* doesn't abort *)
+      inline{1} RO_KEF.extract.
+      if{2}.
+        wp; sp; if.
+          by progress; cut W :
+            (snd pp, (decrypt V.sk (fst pp) V.c, V.t)){2} <>
+            (h, (decrypt V.sk pv c, t)){2}; smt.   
+          by rnd; skip; progress; smt.    
+        skip; progress.
+        cut W :
+         (snd pp, (decrypt V.sk (fst pp) V.c, V.t)){2} <>
+         (h, (decrypt V.sk pv c, t)){2} by smt.
+        by generalize H1; rewrite eq_except_def; smt.    
+    wp; sp; if{1}.
+      by rnd{1}; skip; smt.
+      by skip; smt.
   qed.
   
-  local lemma RCCA_lossless_dec : islossless RCCA(MS_KEM, A(RO_KEF)).O.dec.
+  local lemma RCCA0_lossless_dec : islossless RCCA0.O.dec.
   proof.
     fun.
     sp; if => //.
     inline KEM(RO_KEF, PMS_KEM).dec; wp; sp.
     seq 1 : true => //.
-      by call (_:true) => //; apply lossless_dec.
       by call (_:true ==> true) => //; apply lossless_extract.
   qed.
 
@@ -568,26 +624,20 @@ section.
   proof.
     fun.
     sp; if => //.
-    sp; seq 1 : true => //.
-      by call (_:true); first by apply lossless_dec.
-      sp; if => //.
-        by if => //; wp; try rnd; skip; smt.  
+    sp; if => //.
+    by if => //; wp; try rnd; skip; smt.  
   qed.
 
   local lemma RCCA1_dec_preserves_abort : 
     bd_hoare [ RCCA1.O2.dec : RCCA1.abort ==> RCCA1.abort ] = 1%r.
   proof.
     fun.
-    sp; if => //; wp.
-    seq 3 : RCCA1.abort => //.
-     by call (_:RCCA1.abort); [apply lossless_dec | wp]. 
-     sp; if => //; wp; if. 
-       by rnd; skip; smt.
-       by wp; skip; smt.
-     by bd_hoare; call (_:RCCA1.abort); wp.
+    sp; if => //.
+    sp; if => //.
+    by if => //; wp; try rnd; skip; smt.  
   qed.
   
-  local equiv RCCA_RCCA1_extract :
+  local equiv RCCA0_RCCA1_extract :
     RO_KEF.extract ~ RCCA1.O1.extract :
     !RCCA1.abort{2} /\
     ={p, s} /\ 
@@ -621,8 +671,8 @@ section.
         by skip; smt.
   qed.
   
-  local equiv RCCA_RCCA1_dec :
-    RCCA(MS_KEM, A(RO_KEF)).O.dec ~ RCCA1.O2.dec :
+  local equiv RCCA0_RCCA1_dec :
+    RCCA0.O.dec ~ RCCA1.O2.dec :
     !RCCA1.abort{2} /\
     ={p, t, c} /\ 
     !V.guess{2} /\
@@ -649,133 +699,57 @@ section.
   proof.
     fun.
     sp; if => //.
-    inline KEM(RO_KEF, PMS_KEM).dec.
-    seq 7 3 :
-     (!RCCA1.abort{2} /\
-      !V.guess{2} /\
-      ={maybe_k, pms, p, t, c} /\
-      (pms = decrypt V.sk pv c){2} /\
-      (pv{2}, h{2}) = p{2} /\
-      t0{1} = t{1} /\
-      p0{1} = p{1} /\
-      sk{1} = W.sk{1} /\
-      c0{1} = c{1} /\
-      (pv, h){1} = p0{1} /\
-      mem t{2} V.labels{2} /\
-      mem p{2} P /\
-      RO_KEF.m{1} = RCCA1.m{2} /\
-      W.sk{1} = V.sk{2} /\
-      W.keys{1} = V.keys{2} /\
-      W.labels{1} = V.labels{2} /\
-      (decrypt V.sk (fst pp) V.c = V.pms){2} /\
-      (forall t, 
-         in_dom (snd pp, (V.pms, t)) RCCA1.m => 
-         RCCA1.abort \/ mem t V.labels){2}).
-      sp; exists * sk{1}, pv{1}, c0{1}; elim *; intros sk pv c.
-      by call (dec_spec_rel sk pv c); skip; progress; smt.
-  
-      inline{1} RO_KEF.extract; wp; sp.
-      if{2}.
-        if => //.
-          by wp; rnd; skip; progress; smt.
-          by wp; skip; progress; smt.
-        if{1}.
-          by rnd{1}; skip; progress; smt.
-          by skip; progress; smt.
+    inline{1} RO_KEF.extract; wp; sp.
+    if{2}.
+      if => //.
+        by wp; rnd; skip; progress; smt.
+        by wp; skip; progress; smt.
+      if{1}.
+        by rnd{1}; skip; progress; smt.
+        by skip; progress; smt.
   qed.
-  
-  (* TODO: workaround for transitivity below *) 
-  local module M = RCCA(MS_KEM, A(RO_KEF)).
-  
-  local equiv RCCA_RCCA1 :
-    RCCA(MS_KEM, A(RO_KEF)).main ~ RCCA1.main : 
-      true ==> !RCCA1.abort{2} => ={res}.
+
+  local equiv RCCA0_RCCA1 :
+    RCCA0.main ~ RCCA1.main : true ==> !RCCA1.abort{2} => ={res}.
   proof.
     fun.
-    swap{1} 9 -3; swap{2} 14 -6.
-    inline KEM(RO_KEF, PMS_KEM).enc.   
-    (* Workaround to swap PMS_KEM.enc *)
-    transitivity{1} {
-      MS_KEM.init();
-      (W.pk, W.sk) = MS_KEM.keygen();
-      W.keys = FSet.empty;
-      W.labels = FSet.empty;
-      (pms, c) = PMS_KEM.enc((), W.pk, fst pp);
-      t = M.A.choose(W.pk);
-      b = ${0,1};
-      valid = !mem t W.labels;
-      k0 = RO_KEF.extract(snd pp, (pms, t));
-      k1 = $key;
-      W.keys = add k0 (add k1 W.keys);
-      b'= M.A.guess(c, b ? k1 : k0);
-    }
-    (true ==> ={b, b', valid})
-    (true ==> !RCCA1.abort{2} => (b = b' /\ valid){1} = (b = b' /\ valid){2}) => //.
-    call (_: ={glob W, RO_KEF.m}).
-      by fun; eqobs_in; progress; smt.
-      by fun; eqobs_in.
-      wp; rnd; wp.
-    call (_: ={glob W, RO_KEF.m}); first by eqobs_in.
-    inline MS_KEM.init KEM(RO_KEF, PMS_KEM).init.
-    swap{1} 7 6; swap{1} 7 6; wp; rnd.
-    swap{1} 9 2; swap{1} [7..9] -2; wp.
-    seq 8 5 : (={glob W, RO_KEF.m} /\ pk{1} = W.pk{2} /\ (pv,h){1} = pp).
-    inline RO_KEF.init; wp; call (_:true).
-      by simplify; eqobs_in; smt.
-    wp; call (_:true); skip; progress.
-    seq 2 2 : 
-      (={glob A, glob W, RO_KEF.m, t, pms} /\ 
-       c0{1} = c{2} /\ (pv, h){1} = pp).
-    admit.
-    skip; smt.
-    (*********************************)   
-    seq 7 8 : 
-     (={b} /\
-      pms{1} = V.pms{2} /\
-      c{1} = V.c{2} /\
+    swap{1} 11 -3; swap{2} 14 -6.
+    seq 8 8 : 
+     (={b} /\ pms{1} = V.pms{2} /\ c{1} = V.c{2} /\ (pv, h){1} = pp /\
       (!RCCA1.abort{2} =>
-       ={glob A} /\
-       t{1} = V.t{2} /\
-       RO_KEF.m{1} = RCCA1.m{2} /\
-       W.sk{1} = V.sk{2} /\
-       W.keys{1} = V.keys{2} /\
-       W.labels{1} = V.labels{2} /\
+       ={glob A} /\ t{1} = V.t{2} /\ RO_KEF.m{1} = RCCA1.m{2} /\
+       W.sk{1} = V.sk{2} /\ W.keys{1} = V.keys{2} /\ W.labels{1} = V.labels{2} /\
        (decrypt V.sk (fst pp) V.c = V.pms){2} /\
-       (forall t,
-        in_dom (snd pp, (V.pms, t)) RCCA1.m => mem t V.labels){2})).
-      wp; rnd; simplify.
+       (forall t, in_dom (snd pp, (V.pms, t)) RCCA1.m => mem t V.labels){2})).
+      rnd; simplify.
       call (_:RCCA1.abort,
-        !V.guess{2} /\
-        RO_KEF.m{1} = RCCA1.m{2} /\
-        W.sk{1} = V.sk{2} /\
-        W.keys{1} = V.keys{2} /\
-        W.labels{1} = V.labels{2} /\
+        !V.guess{2} /\ RO_KEF.m{1} = RCCA1.m{2} /\
+        W.sk{1} = V.sk{2} /\ W.keys{1} = V.keys{2} /\ W.labels{1} = V.labels{2} /\
         (decrypt V.sk (fst pp) V.c = V.pms){2} /\
-        (forall t,
-         in_dom (snd pp, (V.pms, t)) RCCA1.m => 
-         RCCA1.abort \/ mem t V.labels){2}).
+        (forall t, in_dom (snd pp, (V.pms, t)) RCCA1.m => 
+           RCCA1.abort \/ mem t V.labels){2}).
       by apply lossless_choose.
-      by apply RCCA_RCCA1_dec.
-      by progress; apply RCCA_lossless_dec.
+      by apply RCCA0_RCCA1_dec.
+      by progress; apply RCCA0_lossless_dec.
       by apply RCCA1_dec_preserves_abort.
-      by apply RCCA_RCCA1_extract.
+      by apply RCCA0_RCCA1_extract.
       by progress; apply lossless_extract.
       by progress; fun; sp; if; try rnd; skip; smt. 
       seq 2 2 : 
-       (W.pk{1} = pk{2} /\ W.sk{1} = V.sk{2} /\ 
-        RO_KEF.m{1} = Core.empty /\ keypair(W.pk, W.sk){1}).
+       (pk{1} = pk{2} /\ W.sk{1} = V.sk{2} /\ 
+        RO_KEF.m{1} = Core.empty /\ keypair(pk, W.sk){1}).
         inline MS_KEM.init RO_KEF.init MS_KEM.keygen; wp.
-        by call keygen_rel; wp; call (_:true).
-        inline V.init; sp.
-        exists * V.sk{2}, pk{2}; elim *; intros sk pk.
+        by call keygen_spec_rel; wp; call (_:true).
+        inline V.init; sp; exists * V.sk{2}, pk{2}; elim *; intros sk pk.
         by call (enc_spec_rel pk sk (fst pp)); skip; smt.
+
       inline RO_KEF.extract; wp; sp.
       case RCCA1.abort{2}.
         (* abort *)
         call (_:RCCA1.abort, RCCA1.abort{2}).
           by apply lossless_guess.
           by exfalso; smt.
-          by progress; apply RCCA_lossless_dec.
+          by progress; apply RCCA0_lossless_dec.
           by apply RCCA1_dec_preserves_abort.
           by exfalso; smt.
           by progress; apply lossless_extract.
@@ -789,18 +763,16 @@ section.
           rcondt{1} 1; first by intros _; skip; smt.
           call (_:RCCA1.abort,
            V.guess{2} /\
-           W.sk{1} = V.sk{2} /\
-           W.keys{1} = V.keys{2} /\
-           W.labels{1} = V.labels{2} /\
+           W.sk{1} = V.sk{2} /\ W.keys{1} = V.keys{2} /\ W.labels{1} = V.labels{2} /\
            eq_except RO_KEF.m{1} RCCA1.m{2} (snd pp, (V.pms, V.t)){2} /\
            in_dom (snd pp, (V.pms, V.t)){2} RO_KEF.m{1} /\
            mem (proj RO_KEF.m{1}.[(snd pp, (V.pms, V.t))]){2} V.keys{2} /\
            decrypt V.sk{2} (fst pp) V.c{2} = V.pms{2}).
           by apply lossless_guess.
-          by apply RCCA_RCCA1_dec_upto.
-          by progress; apply RCCA_lossless_dec.
+          by apply RCCA0_RCCA1_dec_upto.
+          by progress; apply RCCA0_lossless_dec.
           by apply RCCA1_dec_preserves_abort.
-          by apply RCCA_RCCA1_extract_upto.
+          by apply RCCA0_RCCA1_extract_upto.
           by progress; apply lossless_extract.
           by intros _; fun; sp; if; try rnd; skip; smt.
           wp; case b{1}.
@@ -809,8 +781,8 @@ section.
    
           (* !abort /\ !valid *)  
           call{1} (_:true ==> true).
-            apply (lossless_guess RO_KEF (<:RCCA(MS_KEM, A(RO_KEF)).O)).
-              by apply RCCA_lossless_dec.
+            apply (lossless_guess RO_KEF RCCA0.O).
+              by apply RCCA0_lossless_dec.
               by apply lossless_extract.
           call{2} (_:true ==> true).
             apply (lossless_guess RCCA1.O1 RCCA1.O2).
@@ -837,17 +809,15 @@ section.
     1%r / 2%r + Pr[RCCA1.main() @ &m : RCCA1.abort].
   proof.
    intros &m.
-   apply (Trans _ (Pr[RCCA1.main() @ &m : res \/ RCCA1.abort])).
-     by equiv_deno RCCA_RCCA1; smt.  
+   apply (Trans _ Pr[RCCA0.main() @ &m : res]).
+   equiv_deno RCCA_RCCA0 => //.
+   apply (Trans _ Pr[RCCA1.main() @ &m : res \/ RCCA1.abort]).
+     by equiv_deno RCCA0_RCCA1; smt.  
      by rewrite Pr mu_or; smt.
   qed.
   
   
   (** RCCA1 -> RCCA2 **)
-  
-  op find_ext sk (d:(label, (ms * version * hash * ciphertext)) map) h pms t = 
-   in_dom t d /\ 
-   let (k, pv, h', c) = proj d.[t] in h = h' /\ decrypt sk pv c = pms.
   
   local module RCCA2 = {
     var m : (hash * (pms * label), ms) map
@@ -860,7 +830,8 @@ section.
         var t : label;
         (pms, t) = s;
         if (!in_dom (p, (pms, t)) m) {
-          if (find_ext V.sk d p pms t) {
+          if (in_dom t d /\ 
+              let (ms, pv, h, c) = proj d.[t] in p = h /\ decrypt V.sk pv c = pms) {
             k = let (ms, pv, h, c) = proj d.[t] in ms;
           }
           else k = $key;
@@ -974,7 +945,7 @@ section.
       rcondt{2} 1; first by intros &1; skip; intros &2; progress; smt.
       sp; rcondf{2} 1.
         intros &1; skip; intros &2; progress.
-        rewrite /find_ext; cut W := H1 p{2} pms{2} t{2}; smt.   
+        by cut W := H1 p{2} pms{2} t{2}; smt.   
       wp; rnd; skip; progress.
         by smt.   
         elim H8; clear H8; intros ?.
@@ -1067,96 +1038,60 @@ section.
         RCCA1.m{1}.[(h, (pms, t))] = 
         let (k, pv, h', c) = proj RCCA2.d{2}.[t] in Some k)).
   proof.
-     fun.
-     wp; sp; if => //.
-     inline{1} RCCA1.O1.extract.
-     seq 3 2 :
-      ((pms = decrypt V.sk pv c){1} /\
-       (pv{2}, h{2}) = p{2} /\
-       mem t{1} V.labels{1} /\
-       mem p{1} P /\
-       !in_dom t{2} RCCA2.d{2} /\
-       (pv{1}, h{1}) = p{1} /\
-       maybe_k{1} = None /\
-       ={maybe_k, p, t, c, glob V} /\
-      (V.guess{1} => ={V.t}) /\
-      (decrypt V.sk (fst pp) V.c = V.pms){2} /\ 
-      (RCCA1.abort{1} =>
-       (exists t, in_dom (snd pp, (V.pms, t)) RCCA2.m \/
-       (V.guess /\ in_dom V.t RCCA2.d /\
-        let (k, pv, h, c) = proj RCCA2.d.[V.t] in
-         c <> V.c /\ decrypt V.sk pv c = V.pms)){2}) /\
-      (forall t, in_dom t RCCA2.d => mem t V.labels){2} /\
-      (forall h pms t, 
-       (in_dom (h, (pms, t)) RCCA1.m{1} <=>
-       (in_dom (h, (pms, t)) RCCA2.m{2} \/
-        (in_dom t RCCA2.d{2} /\ 
-         let (k, pv, h', c) = proj RCCA2.d{2}.[t] in 
-          h = h' /\ decrypt V.sk{2} pv c = pms)))) /\
-      (forall h pms t, 
-       (in_dom (h, (pms, t)) RCCA1.m{1} => 
-        in_dom (h, (pms, t)) RCCA2.m{2} => 
-        RCCA1.m{1}.[(h, (pms, t))] = RCCA2.m{2}.[(h, (pms, t))])) /\
-      (forall h pms t, 
-       (in_dom (h, (pms, t)) RCCA1.m{1} => 
-        !in_dom (h, (pms, t)) RCCA2.m{2} => 
-          RCCA1.m{1}.[(h, (pms, t))] = 
-          let (k, pv, h', c) = proj RCCA2.d{2}.[t] in Some k))).
-        sp; wp; exists * V.sk{1}, pv{1}, c{1} ; elim *; intros sk pv c.
-        by call{1} (dec_spec sk pv c); skip; progress; smt.
+    fun.
+    wp; sp; if => //.
+    inline{1} RCCA1.O1.extract.
+    sp; if => //; first by smt.
+      if{1}.
+        if{2}.
+          by exfalso; smt.
+          wp; rnd; skip; progress.
+            by smt.
+            elim H12; clear H12; intros ?.
+            cut X : abortL = true by smt; subst.
+            by elim H; smt.
+            by exists t{2}; right; smt.
+            by smt.
+            case (in_dom (h0, (pms0, t0)) RCCA1.m{1}); first by smt.
+            by intros ?; cut Z : 
+              (h0, (pms0, t0)) =
+              (h{2}, (decrypt V.sk{2} pv{2} c{2}, t{2})); smt.
+            elim H12; clear H12; intros ?; first by smt.
+            case (t0 = t{2}).
+              intros ?; subst; elim H12; clear H12; intros X Y.
+              by generalize Y; rewrite /_.[_] Core.get_setE; smt.
+              intros ?.
+              cut L : (in_dom (h0, (pms0, t0)) RCCA1.m{1}); last by smt.
+              rewrite H1.
+              cut L : (in_dom t0 RCCA2.d{2} /\
+                let (k0, pv0, h', c0) = proj RCCA2.d{2}.[t0] in
+                  h0 = h' /\ decrypt V.sk{2} pv0 c0 = pms0).
+              split; first by smt.
+              by generalize H12; rewrite /_.[_] Core.get_setN; smt.
+            by smt.
+            by smt.
+            by case ((h, (decrypt V.sk pv c, t)){2} = (h0, (pms0, t0))); smt.
     
-        sp; if => //; first by smt.
-        if{1}.
-          if{2}.
-            by exfalso; smt.
-            wp; rnd; skip; progress.
-              by smt.
-              elim H13; clear H13; intros ?.
-              cut X : abortL = true by smt; subst.
-              by elim H2; smt.
-              exists t{2}.
-              by right; smt.
-              by smt.
-              case (in_dom (h0, (pms0, t0)) RCCA1.m{1}); first by smt.
-              by intros ?; cut Z : 
-                (h0, (pms0, t0)) =
-                (h{2}, (decrypt V.sk{2} pv{2} c{2}, t{2})); smt.
-              elim H13; clear H13; intros ?; first by smt.
-              case (t0 = t{2}).
-                intros ?; subst; elim H13; clear H13; intros X Y.
-                by generalize Y; rewrite /_.[_] Core.get_setE; smt.
-                intros ?.
-                cut L : (in_dom (h0, (pms0, t0)) RCCA1.m{1}); last by smt.
-                rewrite H4.
-                cut L : (in_dom t0 RCCA2.d{2} /\
-                  let (k0, pv0, h', c0) = proj RCCA2.d{2}.[t0] in
-                    h0 = h' /\ decrypt V.sk{2} pv0 c0 = pms0).
-                split; first by smt.
-                by generalize H13; rewrite /_.[_] Core.get_setN; smt.
-              by smt.
-              by smt.
-              case ((h, (decrypt V.sk pv c, t)){2} = (h0, (pms0, t0))).
-                by smt.
-                by intros ?; generalize H11; rewrite /_.[_] Core.get_setN; smt.
-      
-        (* similarly *)
-        rcondt{2} 1; first by intros &1; skip; intros &2; progress; smt.
-        wp; skip; progress.
-          by smt.
-          elim H9; clear H9; intros ?.
-          cut X : abortL = true by smt; subst.
-          by elim H2; smt.
-          by exists t{2}; right; smt.         
-          by smt.
-          by smt.
-          elim H9; clear H9; first by smt.
-          case (t0 = t{2}); first by smt.
-            intros ? [? ?].
-            case ((h, (decrypt V.sk pv c, t)){2} = (h0, (pms0, t0))).
-              by smt.
-              intros ?; rewrite H4; right; split; first by smt.
-              by generalize H11; rewrite /_.[_] Core.get_setN; smt.
-          by smt.
+      (* similarly *)
+      rcondt{2} 1; first by intros &1; skip; intros &2; progress; smt.
+      wp; skip; progress.
+        by smt.
+        elim H8; clear H8; intros ?.
+        cut X : abortL = true by smt; subst.
+        by elim H; smt.
+        by exists t{2}; right; smt.         
+        by smt.
+        by smt.
+        elim H8; clear H8; first by smt.
+        case (t0 = t{2}); first by smt.
+          intros ? [? ?].
+          case ((h, (decrypt V.sk pv c, t)){2} = (h0, (pms0, t0))).
+            by smt.
+            intros ?; rewrite H1; right; split; first by smt.
+            by generalize H10; rewrite /_.[_] Core.get_setN; smt.
+        by smt.
+
+      by skip; progress; smt.
   qed.
   
   local equiv RCCA1_RCCA2 :
@@ -1226,7 +1161,7 @@ section.
       by apply RCCA1_RCCA2_dec.
       by apply RCCA1_RCCA2_extract. 
     seq 2 2 : (={pk, V.sk} /\ keypair(pk, V.sk){1}).
-      by call keygen_rel; call (_:true); skip.
+      by call keygen_spec_rel; call (_:true); skip.
       exists * pk{1}, V.sk{1}; elim *; intros pk sk.
       call (enc_spec_rel pk sk (fst pp)).
       by inline V.init; wp; skip; progress; smt.
@@ -1369,21 +1304,78 @@ section.
       return proj maybe_pms;
     }
   }.
+
+  local module O = {
+    fun check(p:unit, k:pms, t:version, c:ciphertext) : bool = {
+      var k' : pms;
+      k' = decrypt PCA.V.sk t c;
+      return (k' = k);
+    }
+  }.
  
+  local module OW_PCA0 = {
+    module B = B(O)
+    
+    fun main() : bool = {
+      var pk : pkey;
+      var t : version;
+      var k, k' : pms;
+      var c : ciphertext;
+      PMS_KEM.init();
+      (pk, PCA.V.sk) = PMS_KEM.keygen();
+      (k, c) = PMS_KEM.enc((), pk, fst pp);
+      t = B.choose(pk);
+      k' = B.guess(c);
+      return (k = k');
+    }
+  }.
+
+  local equiv OW_PCA0_OW_PCA_check :
+    O.check ~ PCA.OW_PCA(PMS_KEM, B).O.check : 
+    ={p, k, t, c} /\ ={glob PCA.V} ==> 
+    ={res} /\ ={glob PCA.V}.
+  proof.
+    fun.
+    wp; exists * PCA.V.sk{2}, t{2}, c{2}; elim *; intros sk pv c.
+    by call{2} (dec_spec sk pv c).
+  qed.
+
+  local equiv OW_PCA0_OW_PCA :
+    OW_PCA0.main ~ PCA.OW_PCA(PMS_KEM, B).main : true ==> ={res}.
+  proof.
+    fun.
+    swap{1} 3 1.
+    inline PCA.OW_PCA(PMS_KEM, B).A.guess OW_PCA0.B.guess.
+    eqobs_in (={glob PCA.V}) true : (={k,k',glob Find, glob PCA.V}).
+    apply OW_PCA0_OW_PCA_check.
+    seq 3 3 : 
+     (={pk, glob PCA.V, glob A, glob Find, t} /\ 
+      t{1} = fst pp /\ keypair(pk, PCA.V.sk){2}).
+    inline PCA.OW_PCA(PMS_KEM, B).A.choose OW_PCA0.B.choose; wp.
+    call (_: ={glob PCA.V, glob Find}) => //.
+      fun.
+      eqobs_in true (={glob PCA.V}) : (={maybe_k, glob Find, glob PCA.V}).
+      apply OW_PCA0_OW_PCA_check.
+      fun.
+      eqobs_in (={glob PCA.V}) true : (={k, glob Find, glob PCA.V}).
+      apply OW_PCA0_OW_PCA_check.
+    by inline V.init; wp; call keygen_spec_rel; call (_:true).
+    exists * PCA.V.sk{1}, pk{1}, t{1}; elim *; intros sk pk t.
+    by call (enc_spec_rel pk sk t).
+  qed.
+
   local lemma check_spec : forall _k _t _c,
     bd_hoare 
-    [ PCA.Wrap(PMS_KEM).check : 
+    [ O.check : 
       k = _k /\ t = _t /\ c = _c ==>
       res <=> _k = decrypt PCA.V.sk _t _c ] = 1%r.
   proof.
-    progress; fun.
-    exists * PCA.V.sk; elim *; intros sk.
-    by call (dec_spec sk _t _c); skip; progress; smt.
+    by progress; fun; wp.
   qed.
   
   local lemma find_any_spec : forall _pv _c,
     bd_hoare 
-    [ Find(PCA.Wrap(PMS_KEM)).find_any : 
+    [ Find(O).find_any : 
       pv = _pv /\ c = _c ==> 
       let pms = decrypt PCA.V.sk _pv _c in
        ((exists h t, in_dom (h, (pms, t)) Find.m) <=> res = Some pms) /\
@@ -1406,7 +1398,7 @@ section.
   
   local lemma find_spec : forall _pv _c _h _t,
     bd_hoare 
-    [ Find(PCA.Wrap(PMS_KEM)).find : 
+    [ Find(O).find : 
       pv = _pv /\ c = _c /\ h = _h /\ t = _t ==> 
       let pms = decrypt PCA.V.sk _pv _c in
        (in_dom (_h, (pms, _t)) Find.m <=> res = Some pms) /\
@@ -1430,16 +1422,18 @@ section.
   qed.
   
   local equiv RCCA2_OW_extract : 
-    RCCA2.O1.extract ~ Find(PCA.Wrap(PMS_KEM)).O1.extract :
+    RCCA2.O1.extract ~ Find(O).O1.extract :
     ={p, s} /\ ={V.keys, V.labels, V.guess, V.t, V.c} /\
     V.sk{1} = PCA.V.sk{2} /\ 
     RCCA2.m{1} = Find.m{2} /\ 
-    RCCA2.d{1} = Find.d{2} 
+    RCCA2.d{1} = Find.d{2} /\
+    decrypt V.sk{1} (fst pp) V.c{1} = V.pms{1}
     ==>
     ={res} /\ ={V.keys, V.labels, V.guess, V.t, V.c} /\
     V.sk{1} = PCA.V.sk{2} /\ 
     RCCA2.m{1} = Find.m{2} /\ 
-    RCCA2.d{1} = Find.d{2}. 
+    RCCA2.d{1} = Find.d{2} /\
+    decrypt V.sk{1} (fst pp) V.c{1} = V.pms{1}. 
   proof.
     fun.
     sp; if => //.
@@ -1448,7 +1442,10 @@ section.
         V.sk{1} = PCA.V.sk{2} /\ 
         RCCA2.m{1} = Find.m{2} /\ 
         RCCA2.d{1} = Find.d{2} /\
-        ((find_ext V.sk RCCA2.d p pms t){1} <=> 
+        decrypt V.sk{1} (fst pp) V.c{1} = V.pms{1} /\ 
+        ((in_dom t RCCA2.d /\ 
+          let (ms, pv, h, c) = proj RCCA2.d.[t] in 
+            p = h /\ decrypt V.sk pv c = pms){1} <=> 
          (in_dom t Find.d /\ p = h /\ found){2})).
         sp; exists * pms{2}, pv{2}, c{2}; elim *; intros pms pv c.
         by call{2} (check_spec pms pv c); skip; progress; smt.
@@ -1457,16 +1454,18 @@ section.
   qed.
   
   local equiv RCCA2_OW_dec : 
-    RCCA2.O2.dec ~ Find(PCA.Wrap(PMS_KEM)).O2.dec :
+    RCCA2.O2.dec ~ Find(O).O2.dec :
     ={p, t, c} /\ ={V.keys, V.labels, V.guess, V.t, V.c} /\
     V.sk{1} = PCA.V.sk{2} /\ 
     RCCA2.m{1} = Find.m{2} /\ 
-    RCCA2.d{1} = Find.d{2} 
+    RCCA2.d{1} = Find.d{2} /\
+    decrypt V.sk{1} (fst pp) V.c{1} = V.pms{1} 
     ==>
     ={res} /\ ={V.keys, V.labels, V.guess, V.t, V.c} /\
     V.sk{1} = PCA.V.sk{2} /\ 
     RCCA2.m{1} = Find.m{2} /\ 
-    RCCA2.d{1} = Find.d{2}. 
+    RCCA2.d{1} = Find.d{2} /\
+    decrypt V.sk{1} (fst pp) V.c{1} = V.pms{1}. 
   proof.
     fun.
     sp; if => //.
@@ -1477,6 +1476,7 @@ section.
       V.sk{1} = PCA.V.sk{2} /\
       RCCA2.m{1} = Find.m{2} /\ 
       RCCA2.d{1} = Find.d{2} /\
+      decrypt V.sk{1} (fst pp) V.c{1} = V.pms{1} /\
       !(V.guess /\ (pv, h) = pp /\ t = V.t /\ V.c = c){1} /\
       ((in_dom (h, (decrypt V.sk pv c, t)) RCCA2.m){1} <=> 
        maybe_pms{2} <> None) /\
@@ -1488,73 +1488,123 @@ section.
         by wp; skip; smt.
         by wp; rnd.
   qed.
-  
+
+  local equiv RCCA2_OW_extract_choose : 
+    RCCA2.O1.extract ~ Find(O).O1.extract :
+    ={p, s} /\ ={V.keys, V.labels, V.guess, V.t} /\ !V.guess{1} /\
+    V.sk{1} = PCA.V.sk{2} /\ 
+    RCCA2.m{1} = Find.m{2} /\ 
+    RCCA2.d{1} = Find.d{2} /\
+    decrypt V.sk{1} (fst pp) V.c{1} = V.pms{1}
+    ==>
+    ={res} /\ ={V.keys, V.labels, V.guess, V.t} /\ !V.guess{1} /\
+    V.sk{1} = PCA.V.sk{2} /\ 
+    RCCA2.m{1} = Find.m{2} /\ 
+    RCCA2.d{1} = Find.d{2} /\
+    decrypt V.sk{1} (fst pp) V.c{1} = V.pms{1}. 
+  proof.
+    fun.
+    sp; if => //.
+      seq 0 2 : 
+       (={pms, t, p, s, V.keys, V.labels, V.guess, V.t} /\ !V.guess{1} /\
+        V.sk{1} = PCA.V.sk{2} /\ 
+        RCCA2.m{1} = Find.m{2} /\ 
+        RCCA2.d{1} = Find.d{2} /\
+        decrypt V.sk{1} (fst pp) V.c{1} = V.pms{1} /\ 
+        ((in_dom t RCCA2.d /\ 
+          let (ms, pv, h, c) = proj RCCA2.d.[t] in 
+            p = h /\ decrypt V.sk pv c = pms){1} <=> 
+         (in_dom t Find.d /\ p = h /\ found){2})).
+        sp; exists * pms{2}, pv{2}, c{2}; elim *; intros pms pv c.
+        by call{2} (check_spec pms pv c); skip; progress; smt.
+        by if => //; wp; try rnd; skip; progress.
+      by wp.
+  qed.
+
+  local equiv RCCA2_OW_dec_choose : 
+    RCCA2.O2.dec ~ Find(O).O2.dec :
+    ={p, t, c} /\ ={V.keys, V.labels, V.guess, V.t} /\
+    !V.guess{1} /\
+    V.sk{1} = PCA.V.sk{2} /\ 
+    RCCA2.m{1} = Find.m{2} /\ 
+    RCCA2.d{1} = Find.d{2} /\
+    decrypt V.sk{1} (fst pp) V.c{1} = V.pms{1} 
+    ==>
+    ={res} /\ ={V.keys, V.labels, V.guess, V.t} /\
+    !V.guess{1} /\
+    V.sk{1} = PCA.V.sk{2} /\ 
+    RCCA2.m{1} = Find.m{2} /\ 
+    RCCA2.d{1} = Find.d{2} /\
+    decrypt V.sk{1} (fst pp) V.c{1} = V.pms{1}. 
+  proof.
+    fun.
+    sp; if => //.
+    sp; if => //; first by smt.
+    seq 0 1 :    
+     (maybe_k{1} = None /\
+      ={maybe_k, pv, h, p, t, c, V.labels, V.keys, V.guess, V.t} /\
+      !V.guess{1} /\
+      V.sk{1} = PCA.V.sk{2} /\
+      RCCA2.m{1} = Find.m{2} /\ 
+      RCCA2.d{1} = Find.d{2} /\
+      decrypt V.sk{1} (fst pp) V.c{1} = V.pms{1} /\
+      !(V.guess /\ (pv, h) = pp /\ t = V.t /\ V.c = c){1} /\
+      ((in_dom (h, (decrypt V.sk pv c, t)) RCCA2.m){1} <=> 
+       maybe_pms{2} <> None) /\
+      (maybe_pms <> None => 
+       maybe_pms = Some (decrypt PCA.V.sk pv c)){2}).
+      sp; exists * pv{2}, c{2}, h{2}, t{2}; elim *; intros pv c h t.
+      by call{2} (find_spec pv c h t); skip; progress; smt.  
+      if => //.
+        by wp; skip; smt.
+        by wp; rnd.
+  qed.
+
   local equiv RCCA2_OW :
-    RCCA2.main ~ PCA.OW_PCA(PMS_KEM, B).main :
+    RCCA2.main ~ OW_PCA0.main :
     true ==> (exists t, in_dom (snd pp, (V.pms, t)) RCCA2.m){1} => res{2}.
   proof.
    fun.
-   (* Workaround to swap PMS_KEM.enc *)
-   transitivity{1} {
-    PMS_KEM.init();
-    (pk, V.sk) = PMS_KEM.keygen();
-    V.init();
-    RCCA2.m = Core.empty;
-    RCCA2.d = Core.empty;
-    V.t = RCCA2.A.choose(pk);
-    (V.pms, V.c) = PMS_KEM.enc((), pk, fst pp);
-    k0 = $key;
-    k1 = $key;
-    V.guess = true;
-    V.keys = add k0 (add k1 V.keys);
-    b' = RCCA2.A.guess(V.c, k0);
-   }
-   (true ==> ={glob V, RCCA2.m, RCCA2.d})
-   (true ==> (exists t, in_dom (snd pp, (V.pms, t)) RCCA2.m){1} => (k = k'){2}) => //.
-   call (_: ={glob V, RCCA2.m, RCCA2.d}).
-    by fun; eqobs_in.
-    by fun; eqobs_in.
-    wp; rnd; rnd; simplify.
-    seq 5 5 : (={glob V, pk, RCCA2.m, RCCA2.d}); first by eqobs_in.
-    seq 2 2 : (={glob A, glob V, pk, RCCA2.m, RCCA2.d}).
-      admit (* swap, but technically dec 'uses' V.c *).
-      by trivial.
-   (*********************************)
-   inline PCA.OW_PCA(PMS_KEM, B).A.choose 
-          PCA.OW_PCA(PMS_KEM, B).A.guess.
-   wp; seq 6 7 : (={pk, glob A, V.keys, V.labels, V.guess, V.t, V.c} /\
-    keypair(pk, V.sk){1} /\
+   inline OW_PCA0.B.choose OW_PCA0.B.guess.
+   swap{2} [4..7] -1; wp.
+   seq 6 7 :
+     (={pk, V.keys, V.labels, V.guess, V.t} /\ !V.guess{1} /\
+      RCCA2.m{1} = Find.m{2} /\ RCCA2.d{1} = Find.d{2} /\
+      V.sk{1} = PCA.V.sk{2} /\ pk0{2} = pk{2} /\
+      V.pms{1} = k{2} /\ V.c{1} = c{2} /\ 
+      (decrypt V.sk (fst pp) V.c = V.pms){1}).
+   seq 5 6 : (={pk, V.keys, V.labels, V.guess, V.t} /\ !V.guess{1} /\
+      RCCA2.m{1} = Find.m{2} /\ RCCA2.d{1} = Find.d{2} /\
+      V.sk{1} = PCA.V.sk{2} /\ pk0{2} = pk{2} /\
+      keypair(pk, V.sk){1}).
+   by inline V.init; wp; call keygen_spec_rel; call (_:true).
+   exists * V.sk{1}, pk{1}; elim *; intros sk pk.
+   call (enc_spec_rel pk sk (fst pp)); wp; skip; progress; smt.
+
+   seq 6 9 : (={pk, V.keys, V.labels, V.guess, V.t, V.c} /\
+    V.sk{1} = PCA.V.sk{2} /\ V.c{2} = c0{2} /\ pk0{2} = pk{2} /\
+    V.pms{1} = k{2} /\ 
+    RCCA2.m{1} = Find.m{2} /\ 
+    RCCA2.d{1} = Find.d{2} /\
+    (decrypt V.sk (fst pp) V.c = V.pms){1}).
+   call (_: ={V.keys, V.labels, V.guess, V.t, V.c} /\
     V.sk{1} = PCA.V.sk{2} /\ 
     RCCA2.m{1} = Find.m{2} /\ 
-    RCCA2.d{1} = Find.d{2}).
-      call (_: ={V.keys, V.labels, V.guess, V.t, V.c} /\
-        V.sk{1} = PCA.V.sk{2} /\ 
-        RCCA2.m{1} = Find.m{2} /\ RCCA2.d{1} = Find.d{2}).
-        by apply RCCA2_OW_dec.
-        by apply RCCA2_OW_extract.
-      inline V.init; wp; call keygen_rel; wp; call (_:true); skip; smt.
-    seq 1 2 :
-     (={pk, glob A, V.keys, V.labels, V.guess, V.t} /\
-      (decrypt V.sk (fst pp) V.c = V.pms){1} /\
-      V.pms{1} = k{2} /\ V.c{1} = c{2} /\
-      V.sk{1} = PCA.V.sk{2} /\ 
-      RCCA2.m{1} = Find.m{2} /\ RCCA2.d{1} = Find.d{2}).
-      exists * V.sk{1}, pk{1}; elim *; intros sk pk.
-      by call (enc_spec_rel pk sk (fst pp)); wp; skip; smt.  
-    seq 5 7 : (={pk, glob A, V.keys, V.labels, V.guess, V.t, V.c} /\ 
-     V.sk{1} = PCA.V.sk{2} /\ 
-     V.pms{1} = k{2} /\
-     (decrypt V.sk (fst pp) V.c = V.pms){1} /\
-     V.pms{1} = k{2} /\ V.c{1} = c0{2} /\
-     RCCA2.m{1} = Find.m{2} /\ RCCA2.d{1} = Find.d{2}).
-     call (_: ={V.keys, V.labels, V.guess, V.t, V.c} /\
-      V.sk{1} = PCA.V.sk{2} /\ 
-      RCCA2.m{1} = Find.m{2} /\ 
-      RCCA2.d{1} = Find.d{2}).
-       by apply RCCA2_OW_dec.
-       by apply RCCA2_OW_extract.
-     by wp; rnd; rnd; wp.  
-    exists * c0{2}; elim *; intros c.
+    RCCA2.d{1} = Find.d{2} /\
+    (decrypt V.sk (fst pp) V.c = V.pms){1}).
+     by apply RCCA2_OW_dec.
+     by apply RCCA2_OW_extract.
+    wp; rnd; rnd; wp.
+   call (_: ={V.keys, V.labels, V.guess, V.t} /\ !V.guess{1} /\
+    V.sk{1} = PCA.V.sk{2} /\ 
+    RCCA2.m{1} = Find.m{2} /\ 
+    RCCA2.d{1} = Find.d{2} /\
+    (decrypt V.sk (fst pp) V.c = V.pms){1}).
+     by apply RCCA2_OW_dec_choose.
+     by apply RCCA2_OW_extract_choose.
+   skip; progress.
+
+    wp; exists * c0{2}; elim *; intros c.
     call{2} (find_any_spec (fst pp) c).
     by wp; skip; progress; smt.
   qed.
@@ -1563,7 +1613,10 @@ section.
     Pr[RCCA2.main() @ &m : exists t, in_dom (snd pp, (V.pms, t)) RCCA2.m] <=
     Pr[PCA.OW_PCA(PMS_KEM, B).main() @ &m : res].
   proof.
-    by intros &m; equiv_deno RCCA2_OW.
+    intros &m.
+    apply (Trans _ Pr[OW_PCA0.main() @ &m : res]).
+    by equiv_deno RCCA2_OW.
+    by equiv_deno OW_PCA0_OW_PCA.
   qed.
   
   
@@ -1595,72 +1648,102 @@ section.
       return let (k, pv, h, c) = proj Find.d.[V.t] in (pv, c);
     }
   }.
+
+  local module NR_PCA0 = {
+    module C = C(O)
+    
+    fun main() : bool = {
+      var pk : pkey;
+      var t, t' : version;
+      var k, k' : pms;
+      var c, c' : ciphertext;
+      PMS_KEM.init();
+      (pk, PCA.V.sk) = PMS_KEM.keygen();
+      (k, c) = PMS_KEM.enc((), pk, fst pp);
+      t = C.choose(pk);
+      (t', c') = C.guess(c);
+      k' = PMS_KEM.dec((), PCA.V.sk, t', c');
+      return (c <> c' /\ k' = k);
+    }
+  }.
+
+  local equiv NR_PCA0_NR_PCA :
+    NR_PCA0.main ~ PCA.NR_PCA(PMS_KEM, C).main : true ==> ={res}.
+  proof.
+    fun.
+    swap{1} 3 1.
+    inline PCA.NR_PCA(PMS_KEM, C).A.guess NR_PCA0.C.guess.
+    call (_: ={glob Find, glob PCA.V}); wp.
+    call (_: ={glob Find, glob PCA.V}).
+      fun.
+      eqobs_in true (={glob PCA.V}) : (={maybe_k, glob Find, glob PCA.V}).
+      apply OW_PCA0_OW_PCA_check.
+      fun.
+      eqobs_in (={glob PCA.V}) true : (={k, glob Find, glob PCA.V}).
+      apply OW_PCA0_OW_PCA_check.
+    seq 3 3 : 
+     (={pk, glob PCA.V, glob A, glob Find, t} /\ 
+      t{1} = fst pp /\ keypair(pk, PCA.V.sk){2}).
+    inline PCA.NR_PCA(PMS_KEM, C).A.choose NR_PCA0.C.choose; wp.
+    call (_: ={glob PCA.V, glob Find}) => //.
+      fun.
+      eqobs_in true (={glob PCA.V}) : (={maybe_k, glob Find, glob PCA.V}).
+      apply OW_PCA0_OW_PCA_check.
+      fun.
+      eqobs_in (={glob PCA.V}) true : (={k, glob Find, glob PCA.V}).
+      apply OW_PCA0_OW_PCA_check.
+    by inline V.init; wp; call keygen_spec_rel; call (_:true).
+    wp; rnd; rnd; wp.
+    exists * PCA.V.sk{1}, pk{1}, t{1}; elim *; intros sk pk t.
+    by call (enc_spec_rel pk sk t); skip; progress; smt.
+  qed.
   
   local equiv RCCA2_NR :
-    RCCA2.main ~ PCA.NR_PCA(PMS_KEM, C).main :
+    RCCA2.main ~ NR_PCA0.main :
     true ==> 
     (let (k, pv, h, c) = proj RCCA2.d.[V.t] in
        c <> V.c /\ decrypt V.sk pv c = V.pms){1} => res{2}.
   proof.
    fun.
-   (* Workaround to swap PMS_KEM.enc *)
-   transitivity {1} {
-     PMS_KEM.init();
-     (pk, V.sk) = PMS_KEM.keygen();
-     V.init();
-     RCCA2.m = Core.empty;
-     RCCA2.d = Core.empty;
-     V.t = RCCA2.A.choose(pk);
-     (V.pms, V.c) = PMS_KEM.enc((), pk, fst pp);
-     k0 = $key;
-     k1 = $key;
-     V.guess = true;
-     V.keys = add k0 (add k1 V.keys);
-     b' = RCCA2.A.guess(V.c, k0);
-   }
-   (true ==> ={glob V, RCCA2.m, RCCA2.d})
-   (true ==> 
-    (let (k, pv, h, c) = proj RCCA2.d.[V.t] in
-     c <> V.c /\ decrypt V.sk pv c = V.pms){1} => (c <> c' /\ k' = k){2}) => //.
-   call (_: ={glob V, RCCA2.m, RCCA2.d}).
-     by fun; eqobs_in.
-     by fun; eqobs_in.
-    wp; rnd; rnd; simplify.
-    seq 5 5 : (={glob V, pk, RCCA2.m, RCCA2.d}); first by eqobs_in.
-    seq 2 2 : (={glob A, glob V, pk, RCCA2.m, RCCA2.d}).
-      admit (* swap, but technically dec 'uses' V.c *).
-      by skip.
-   (*********************************)
-   inline PCA.NR_PCA(PMS_KEM, C).A.choose 
-          PCA.NR_PCA(PMS_KEM, C).A.guess.
-   wp; seq 6 7 : (={pk, glob A, V.keys, V.labels, V.guess, V.t, V.c} /\
-    keypair(pk, V.sk){1} /\
+   inline NR_PCA0.C.choose NR_PCA0.C.guess.
+   swap{2} [4..7] -1; wp.
+   seq 6 7 :
+     (={pk, V.keys, V.labels, V.guess, V.t} /\ !V.guess{1} /\
+      RCCA2.m{1} = Find.m{2} /\ RCCA2.d{1} = Find.d{2} /\
+      V.sk{1} = PCA.V.sk{2} /\ pk0{2} = pk{2} /\
+      V.pms{1} = k{2} /\ V.c{1} = c{2} /\ 
+      (decrypt V.sk (fst pp) V.c = V.pms){1}).
+   seq 5 6 : (={pk, V.keys, V.labels, V.guess, V.t} /\ !V.guess{1} /\
+      RCCA2.m{1} = Find.m{2} /\ RCCA2.d{1} = Find.d{2} /\
+      V.sk{1} = PCA.V.sk{2} /\ pk0{2} = pk{2} /\
+      keypair(pk, V.sk){1}).
+   by inline V.init; wp; call keygen_spec_rel; call (_:true).
+   exists * V.sk{1}, pk{1}; elim *; intros sk pk.
+   call (enc_spec_rel pk sk (fst pp)); wp; skip; progress; smt.
+
+   seq 6 9 : (={pk, V.keys, V.labels, V.guess, V.t, V.c} /\
+    V.sk{1} = PCA.V.sk{2} /\ V.c{2} = c0{2} /\ c{2} = c0{2} /\ pk0{2} = pk{2} /\
+    V.pms{1} = k{2} /\ 
+    RCCA2.m{1} = Find.m{2} /\ 
+    RCCA2.d{1} = Find.d{2} /\
+    (decrypt V.sk (fst pp) V.c = V.pms){1}).
+   call (_: ={V.keys, V.labels, V.guess, V.t, V.c} /\
     V.sk{1} = PCA.V.sk{2} /\ 
-    RCCA2.m{1} = Find.m{2} /\ RCCA2.d{1} = Find.d{2}).
-    call (_: ={V.keys, V.labels, V.guess, V.t, V.c} /\
-     V.sk{1} = PCA.V.sk{2} /\ 
-     RCCA2.m{1} = Find.m{2} /\ RCCA2.d{1} = Find.d{2}).
+    RCCA2.m{1} = Find.m{2} /\ 
+    RCCA2.d{1} = Find.d{2} /\
+    (decrypt V.sk (fst pp) V.c = V.pms){1}).
      by apply RCCA2_OW_dec.
      by apply RCCA2_OW_extract.
-    by inline V.init; wp; call keygen_rel; wp; call (_:true); skip; smt.
-  
-    seq 6 9 : (={b', pk, glob A, V.keys, V.labels, V.guess, V.t, V.c} /\
-     V.sk{1} = PCA.V.sk{2} /\ 
-     V.c{1} = c{2} /\ V.pms{1} = k{2} /\
-     (decrypt V.sk (fst pp) V.c = V.pms){1} /\
-     RCCA2.m{1} = Find.m{2} /\ RCCA2.d{1} = Find.d{2}). 
-    call (_: ={V.keys, V.labels, V.guess, V.t, V.c} /\
-     V.sk{1} = PCA.V.sk{2} /\ 
-     RCCA2.m{1} = Find.m{2} /\ 
-     RCCA2.d{1} = Find.d{2}).
-      by apply RCCA2_OW_dec.
-      by apply RCCA2_OW_extract.
-  
     wp; rnd; rnd; wp.
-    exists * V.sk{1}, pk{1}; elim *; intros sk pk.
-    call (enc_spec_rel pk sk (fst pp)).
-    wp; skip; progress; smt.
-  
+   call (_: ={V.keys, V.labels, V.guess, V.t} /\ !V.guess{1} /\
+    V.sk{1} = PCA.V.sk{2} /\ 
+    RCCA2.m{1} = Find.m{2} /\ 
+    RCCA2.d{1} = Find.d{2} /\
+    (decrypt V.sk (fst pp) V.c = V.pms){1}).
+     by apply RCCA2_OW_dec_choose.
+     by apply RCCA2_OW_extract_choose.
+   skip; progress.
+
     sp; wp; exists * PCA.V.sk{2}, t'{2}, c'{2}; elim *; intros sk pv c.
     call{2} (dec_spec sk pv c).
     by skip; progress; smt.
@@ -1671,7 +1754,10 @@ section.
        c <> V.c /\ decrypt V.sk pv c = V.pms] <=
     Pr[PCA.NR_PCA(PMS_KEM, C).main() @ &m : res].
   proof.
-    by intros &m; equiv_deno RCCA2_NR.
+    intros &m.
+    apply (Trans _ Pr[NR_PCA0.main() @ &m : res]).
+    by equiv_deno RCCA2_NR.
+    by equiv_deno NR_PCA0_NR_PCA.
   qed.
   
   (** Conclusion **)
